proofs/lean/SatSolver/Extraction/FunsExternal_Template.lean
@@ -52,17 +52,8 @@ axiom cnf.Cnf.Insts.CoreFmtDebug.fmt
     core.fmt.Error) × core.fmt.Formatter × (core.fmt.Formatter →
     core.fmt.Formatter))
 
-/-- [sat_solver::expr::{impl core::fmt::Debug for sat_solver::expr::Entry}::fmt]:
-    Source: 'src/expr.rs', lines 11:9-11:14
-    Visibility: public -/
-axiom expr.Entry.Insts.CoreFmtDebug.fmt
-  :
-  expr.Entry → core.fmt.Formatter → RustM ((core.result.Result Unit
-    core.fmt.Error) × core.fmt.Formatter × (core.fmt.Formatter →
-    core.fmt.Formatter))
-
 /-- [sat_solver::expr::{impl core::fmt::Debug for sat_solver::expr::Map}::fmt]:
-    Source: 'src/expr.rs', lines 17:9-17:14
+    Source: 'src/expr.rs', lines 24:9-24:14
     Visibility: public -/
 axiom expr.Map.Insts.CoreFmtDebug.fmt
   :
@@ -71,7 +62,7 @@ axiom expr.Map.Insts.CoreFmtDebug.fmt
     core.fmt.Formatter))
 
 /-- [sat_solver::expr::{impl core::fmt::Debug for sat_solver::expr::Expr}::fmt]:
-    Source: 'src/expr.rs', lines 45:9-45:14
+    Source: 'src/expr.rs', lines 52:9-52:14
     Visibility: public -/
 axiom expr.Expr.Insts.CoreFmtDebug.fmt
   :
@@ -80,7 +71,7 @@ axiom expr.Expr.Insts.CoreFmtDebug.fmt
     core.fmt.Formatter))
 
 /-- [sat_solver::expr::{impl core::fmt::Display for sat_solver::expr::Expr}::fmt]:
-    Source: 'src/expr.rs', lines 56:4-71:5
+    Source: 'src/expr.rs', lines 63:4-78:5
     Visibility: public -/
 axiom expr.Expr.Insts.CoreFmtDisplay.fmt
   :
